Change constructors names to snake case

LocalLang/Typing.lean
@@ -5,17 +5,17 @@ import LocalLang.Types
 
 mutual
   inductive TypeJdg : TypeContext → Expr → LLType → Prop where
-    | jdgVar {Γ : TypeContext}  {name : String} {ty : LLType} (H : Γ[name]? = some ty)
+    | jdg_var {Γ : TypeContext}  {name : String} {ty : LLType} (H : Γ[name]? = some ty)
                       : TypeJdg Γ (.var name) ty
-    | jdgConst {Γ : TypeContext} {n : ℕ} : TypeJdg Γ (.const n) LLType.nat
-    | jdgFun {f} {Γ : TypeContext} {es : List Expr} {arg_types : List LLType} {T_return : LLType}
+    | jdg_const {Γ : TypeContext} {n : ℕ} : TypeJdg Γ (.const n) LLType.nat
+    | jdg_fun {f} {Γ : TypeContext} {es : List Expr} {arg_types : List LLType} {T_return : LLType}
                   (H_f : Γ[f]? = some (.func arg_types T_return))
                   (H_args : TypeJdgList Γ es arg_types)
                         : TypeJdg Γ (.funCall f es) (LLType.func arg_types T_return)
-    | jdgBinOp {Γ : TypeContext} {op : BinOp} {e₁ e₂ : Expr}
+    | jdg_binOp {Γ : TypeContext} {op : BinOp} {e₁ e₂ : Expr}
                 (H₁ : TypeJdg Γ e₁ LLType.nat) (H₂ : TypeJdg Γ e₂ LLType.nat)
                         : TypeJdg Γ (.binOp op e₁ e₂) .nat
-    | jdgLetIn {Γ : TypeContext} {name : String} {e₁ e₂ : Expr} {ty₁ ty₂ : LLType}
+    | jdg_let_in {Γ : TypeContext} {name : String} {e₁ e₂ : Expr} {ty₁ ty₂ : LLType}
                 (H₁ : TypeJdg Γ e₁ ty₁)
                 (H₂ : TypeJdg (Γ.insert name ty₁) e₂ ty₂)
                         : TypeJdg  Γ (.letIn name e₁ e₂) ty₂
