LocalLang/TypingExamples.lean
@@ -2,15 +2,15 @@ import LocalLang.Typing
 
 -- Examples for TypeJdg
 example : TypeJdg {} (.const 5) .nat := by
-  apply TypeJdg.jdgConst
+  apply TypeJdg.jdg_const
 
 example : TypeJdg {("x", .nat)} (.var "x") .nat := by
-  apply TypeJdg.jdgVar
+  apply TypeJdg.jdg_var
   simp
 
 def ctx : TypeContext := {("add", .func [.nat] .nat), ("x", .nat)}
 
 example : TypeJdg ctx (.funCall "add" [.var "x"]) (LLType.func [.nat] .nat) := by
-  apply TypeJdg.jdgFun
+  apply TypeJdg.jdg_fun
   · simp [ctx]
   · sorry
